During these problems you'll be using the [[Trigonometric Identities]] and multiplying by 1

## Examples
Referenced From [[VerifyingTrigIdentitiesProblems]]
### 1)
$(sin\theta-cos\theta)(sec\theta+csc\theta)=tan\theta-cot\theta$
$(sin\theta-cos\theta)(sec\theta+csc\theta)=$
$(\frac{sin\theta}{1}-\frac{cos\theta}{1})(\frac{1}{cos\theta}+\frac{1}{sin\theta})=$ Reciprocal Identity
$\frac{sin\theta}{cos\theta}+\frac{sin\theta}{sin\theta}-\frac{cos\theta}{cos\theta}-\frac{cos\theta}{sin\theta}=$ Distribute out
$tan\theta+1-1-cot\theta=$ Quotient Identity 
$tan\theta-cot\theta=$ Answer

### 2)
#### $\frac{cot(x)-tan(x)}{cot(x)+tan(x)}=cos(2x)$ Question
#### $\frac{\frac{cos(x)}{sin(x)}-\frac{sin(x)}{cos(x)}}{\frac{cos(x)}{sin(x)}+\frac{sin(x)}{cos(x)}}=$ Used the [[Quotient Identities]]
#### $\frac{\frac{cos^2x-sin^2x}{sinxcosx}}{\frac{cos^2x+sin^2x}{sinxcosx}}=$ Multiply out denominators so we can subtract fractions
#### $\frac{cos^2x-sin^2x}{sinxcosx}*\frac{sinxcosx}{cos^2x+sin^2x}$ Copy dot flip to rewrite [[Division]]
#### $\frac{cos^2x-sin^2x}{cos^2x+sin^2x}=$ cancel out $sinxcosx$ from numerator and denominator
#### $\frac{cos2x}{cos^2x+sin^2x}=$ Used [[Double Angle Formula]]
#### $\frac{cos2x}{1}=$ Used [[Pythagorean Identities]] to convert denominator to 1
#### $cos2x=$ Answer

![[VerifyingTriIdentity2.png]]





